theories/rules/rules_base.v
@@ -1001,6 +1001,7 @@ Definition regs_of (i: instr): gset RegName :=
   | GetWType dst src => {[ dst; src ]}
   | Add r arg1 arg2 => {[ r ]} ∪ regs_of_argument arg1 ∪ regs_of_argument arg2
   | Sub r arg1 arg2 => {[ r ]} ∪ regs_of_argument arg1 ∪ regs_of_argument arg2
+  | Mod r arg1 arg2 => {[ r ]} ∪ regs_of_argument arg1 ∪ regs_of_argument arg2
   | Lt r arg1 arg2 => {[ r ]} ∪ regs_of_argument arg1 ∪ regs_of_argument arg2
   | Mov r arg => {[ r ]} ∪ regs_of_argument arg
   | Restrict r1 arg => {[ r1 ]} ∪ regs_of_argument arg
